rt refine: misc Schedule_R.thy corres lemmas
Signed-off-by: Mitchell Buckley <mitchell.alan.buckley@gmail.com>

proof/refine/ARM/Schedule_R.thy
@@ -3865,6 +3865,217 @@ lemma awaken_corres:
   apply (fastforce intro!: awaken_terminates)
   done
 
+(* FIXME: Many of these can be moved higher? *)
+lemma getReprogramTimer_corres:
+  "corres (=) \<top> \<top> (gets reprogram_timer) getReprogramTimer"
+  by (clarsimp simp: getReprogramTimer_def state_relation_def)
+
+lemma setDomainTime_corres:
+  "dt = dt' \<Longrightarrow>
+  corres dc \<top> \<top> (modify (domain_time_update (\<lambda>_. dt))) (setDomainTime dt')"
+  apply (clarsimp simp: setDomainTime_def, rule corres_modify)
+  by (clarsimp simp: state_relation_def swp_def)
+
+lemma setConsumedTime_corres:
+  "ct = ct' \<Longrightarrow>
+  corres dc \<top> \<top> (modify (consumed_time_update (\<lambda>_. ct))) (setConsumedTime ct')"
+  apply (clarsimp simp: setConsumedTime_def, rule corres_modify)
+  by (clarsimp simp: state_relation_def swp_def)
+
+lemma setCurSc_corres:
+  "sc = sc' \<Longrightarrow>
+   corres dc \<top> \<top> (modify (cur_sc_update (\<lambda>_. sc))) (setCurSc sc')"
+  apply (clarsimp simp: setCurSc_def, rule corres_modify)
+  by (clarsimp simp: state_relation_def swp_def)
+
+lemma machine_op_lift_corres_trivial:
+  "f = f' \<Longrightarrow> corres_underlying Id False True dc \<top> \<top> (machine_op_lift f) (machine_op_lift f')"
+  unfolding setDeadline_def
+  apply (clarsimp simp: machine_op_lift_def machine_rest_lift_def)
+  apply (rule corres_guard_imp)
+    apply (rule corres_split [OF corres_gets_trivial], simp)
+      apply (rule corres_split_eqr [OF _ corres_select_f])
+          apply (clarsimp, rule corres_modify, simp)
+         apply (clarsimp simp: ignore_failure_def)
+        apply (clarsimp simp: ignore_failure_def)
+       apply wpsimp+
+  done
+
+lemma setDeadline_corres:
+  "dl = dl' \<Longrightarrow> corres_underlying Id False True dc \<top> \<top> (setDeadline dl) (setDeadline dl')"
+  unfolding setDeadline_def
+  by (rule machine_op_lift_corres_trivial, simp)
+
+(* Most sched contexts should satisfy these conditions. The lemma below (standard_sc_common_usage)
+   illustrates a common situation where these conditions hold *)
+abbreviation standard_sc where
+  "standard_sc sc \<equiv> scRefillMax sc \<le> length (scRefills sc) \<and> scRefillHead sc < scRefillMax sc \<and>
+                    scRefillCount sc \<le> scRefillMax sc \<and> 0 < scRefillCount sc"
+
+lemma standard_sc_common_usage:
+  "\<exists>n. sc_relation sc n sc' \<Longrightarrow> sc_active sc \<Longrightarrow> sc_valid_refills sc \<Longrightarrow> valid_sched_context' sc' s'
+   \<Longrightarrow> standard_sc sc'"
+  apply (clarsimp simp: sc_valid_refills_def valid_sched_context'_def active_sc_def sc_relation_def)
+  apply (cases "scRefillCount sc' = 0"; simp)
+  apply (subgoal_tac "sc_refills sc = []")
+   apply (clarsimp split: if_splits simp: rr_valid_refills_def sp_valid_refills_def)
+  apply (clarsimp simp: refills_map_def)
+  done
+
+lemma refillSingle_equiv:
+  "standard_sc sca \<Longrightarrow>
+   (length (refills_map (scRefillHead sca) (scRefillCount sca) (scRefillMax sca) (scRefills sca)) = Suc 0)
+    = (scRefillHead sca = refillTailIndex sca)"
+  apply (clarsimp simp: valid_sched_context'_def refillTailIndex_def refills_map_def)
+  apply (case_tac "scRefillCount sca = Suc 0"; simp)
+  apply (auto simp: Let_def)
+  done
+
+lemma refillSingle_corres:
+  "scp = scp' \<Longrightarrow>
+   corres (=) (sc_at scp) (sc_at' scp' and (\<lambda>s. obj_at' standard_sc scp' s))
+     (refill_single scp) 
+     (refillSingle scp')"
+  unfolding refill_single_def refillSingle_def
+  apply (simp add: refill_size_def get_refills_def)
+  apply (rule stronger_corres_guard_imp)
+    apply (rule_tac R'="\<lambda>sc s. standard_sc sc" and R="\<lambda>_ _ . True" in corres_split)
+       apply (rule get_sc_corres)
+      apply (clarsimp simp: sc_relation_def)
+      apply (rule refillSingle_equiv; simp)
+     apply wpsimp+
+  apply (clarsimp simp: obj_at'_def)
+  done
+
+lemma sc_relation_refill_hd_equiv:
+  "\<exists>n. sc_relation rv n rv' \<Longrightarrow> standard_sc rv' \<Longrightarrow> refill_hd rv = refill_map (refillHd rv')"
+  apply (subgoal_tac " sc_refills rv \<noteq> []")
+   apply (clarsimp simp: sc_relation_def refillHd_def refills_map_def valid_sched_context'_def hd_map hd_wrap_slice refill_map_def)
+  apply (clarsimp simp: sc_relation_def refills_map_def)
+  apply (subgoal_tac "length (wrap_slice (scRefillHead rv') (scRefillCount rv') (scRefillMax rv') (scRefills rv')) = scRefillCount rv'")
+   apply (clarsimp simp: refills_map_def)
+  apply (rule length_wrap_slice; simp)
+  done
+
+lemma pspace_relation_sc_relation:
+  "pspace_relation h h' \<Longrightarrow> 
+   h x = Some (kernel_object.SchedContext sc n) \<Longrightarrow>
+   h' x = Some (KOSchedContext sc') \<Longrightarrow>
+   valid_sched_context_size n \<Longrightarrow>
+   sc_relation sc n sc'"
+  apply (clarsimp simp: pspace_relation_def)
+  apply (drule_tac x=x in bspec, clarsimp)
+  by (clarsimp)
+
+lemma pspace_relation_tcb_relation:
+  "pspace_relation h h' \<Longrightarrow> 
+   h x = Some (kernel_object.TCB tcb) \<Longrightarrow>
+   h' x = Some (KOTCB tcb') \<Longrightarrow>
+   tcb_relation tcb tcb'"
+  apply (clarsimp simp: pspace_relation_def)
+  apply (drule_tac x=x in bspec, clarsimp)
+  by (clarsimp simp: other_obj_relation_def)
+
+(* This is not particularly insightful, it just shortens setNextInterrupt_corres *)
+lemma setNextInterrupt_corres_helper:
+  "\<lbrakk>valid_objs' s'; (s, s') \<in> state_relation; active_sc_tcb_at t s;
+    valid_objs s; active_sc_valid_refills s; pspace_aligned s; pspace_distinct s\<rbrakk>
+    \<Longrightarrow> \<exists>tcb. ko_at' tcb t s' \<and> sc_at' (the (tcbSchedContext tcb)) s' \<and>
+        (\<forall>ko. ko_at' ko (the (tcbSchedContext tcb)) s' \<longrightarrow> standard_sc ko)"
+  apply (subgoal_tac "\<exists>tcb'. ko_at' (tcb'  :: tcb) t s'", clarsimp)
+   apply (clarsimp simp: pred_map_def vs_all_heap_simps)
+   apply (rename_tac tcb' scp tcb sc n)
+   apply (frule pspace_relation_tcb_relation [OF state_relation_pspace_relation], assumption)
+    apply (clarsimp simp: obj_at'_def projectKOs, rule refl)
+   apply (rule_tac x=tcb' in exI, simp)
+   apply (prop_tac "tcbSchedContext tcb' = Some scp", clarsimp simp: tcb_relation_def, simp)
+   apply (subgoal_tac "sc_at' scp s'", clarsimp)
+    apply (frule pspace_relation_sc_relation[OF state_relation_pspace_relation], assumption)
+      apply (clarsimp simp: obj_at'_def projectKOs, rule refl)
+     apply (erule (1) valid_sched_context_size_objsI)
+    apply (rule standard_sc_common_usage, erule exI)
+      apply (clarsimp simp: active_sc_def vs_all_heap_simps pred_map_def is_tcb obj_at_def)
+     apply (subgoal_tac "valid_refills scp s", clarsimp simp: valid_refills_def2 obj_at_def)
+     apply (erule active_sc_valid_refillsE[rotated])
+     apply (clarsimp simp: active_sc_def vs_all_heap_simps pred_map_def is_tcb obj_at_def)
+    apply (frule (1) sc_ko_at_valid_objs_valid_sc', clarsimp, assumption)
+   apply (erule cross_relF [OF _ sc_at'_cross_rel], clarsimp simp: obj_at_def is_sc_obj)
+   apply (erule (1) valid_sched_context_size_objsI)
+  apply (subgoal_tac "tcb_at t s")
+   apply (frule cross_relF [OF _ tcb_at'_cross_rel], clarsimp, assumption)
+   apply (clarsimp simp: obj_at'_def projectKOs)
+  apply (clarsimp simp: obj_at_def vs_all_heap_simps pred_map_def is_tcb)
+  done
+
+lemma setNextInterrupt_corres:
+  "corres dc ((\<lambda>s. active_sc_tcb_at (cur_thread s) s) and valid_release_q and valid_objs
+              and active_sc_valid_refills and pspace_aligned and pspace_distinct) 
+             valid_objs'
+             set_next_interrupt 
+             setNextInterrupt"
+  unfolding setNextInterrupt_def set_next_interrupt_def
+  apply (rule stronger_corres_guard_imp)
+    apply (rule corres_split [OF getCurTime_corres])
+      apply (rule corres_split [OF gct_corres], simp)
+        apply (rule corres_split_eqr [OF _ get_tcb_obj_ref_corres])
+           apply (rule corres_assert_opt_assume_l)
+           apply (rule corres_split [OF get_sc_corres])
+             apply (rule_tac F="standard_sc rv'" in corres_gen_asm2)
+             apply (rule corres_split [OF corres_if])
+                  apply (clarsimp simp: num_domains_def numDomains_def)
+                 apply (rule corres_split [OF domain_time_corres])
+                   apply (simp only: fun_app_def)
+                   apply (rule corres_return_eq_same)
+                   apply (simp add: sc_relation_refill_hd_equiv refill_map_def)
+                  apply wpsimp
+                 apply wpsimp
+                apply (rule corres_return_eq_same)
+                apply (simp add: sc_relation_refill_hd_equiv refill_map_def)
+               apply (rule corres_split [OF getReleaseQueue_corres])
+                 apply (rule corres_split [OF corres_if], simp)
+                     apply (rule corres_return_eq_same, simp)
+                    apply (rule corres_split_eqr)
+                       apply (rule corres_assert_opt_assume_l)
+                       apply (simp)
+                       apply (rule corres_split [OF get_sc_corres])
+                         apply (rule_tac F="standard_sc rv'c" in corres_gen_asm2)
+                         apply (rule corres_return_eq_same)
+                         apply (simp add: sc_relation_refill_hd_equiv refill_map_def)
+                        apply wpsimp
+                       apply wpsimp
+                      apply (simp, rule get_tcb_obj_ref_corres)
+                      apply (clarsimp simp: tcb_relation_def)
+                     apply (wpsimp wp: get_tcb_obj_ref_wp)
+                    apply (wpsimp wp: threadGet_wp)
+                   apply (rule corres_machine_op)
+                   apply (simp only:, rule setDeadline_corres, simp)
+                  apply wpsimp+
+          apply (clarsimp simp: tcb_relation_def)
+         apply (wpsimp wp: get_tcb_obj_ref_wp)
+        apply (wpsimp wp: threadGet_wp)
+       apply wpsimp+
+   apply (subgoal_tac "release_queue s \<noteq> [] \<longrightarrow> active_sc_tcb_at (hd (release_queue s)) s")
+    apply (fastforce simp: cur_tcb_def pred_tcb_at_def vs_all_heap_simps obj_at_def is_sc_obj is_tcb
+                     elim: valid_sched_context_size_objsI)[1]
+   apply (clarsimp simp: valid_release_q_def)
+  apply simp
+  apply (subgoal_tac "(\<exists>tcb. ko_at' tcb (ksCurThread s') s' \<and>
+                    sc_at' (the (tcbSchedContext tcb)) s' \<and>
+                    (\<forall>ko. ko_at' ko (the (tcbSchedContext tcb)) s' \<longrightarrow> standard_sc ko)) \<and> (ksReleaseQueue s' \<noteq> [] \<longrightarrow> (\<exists>tcb. ko_at' tcb (hd (ksReleaseQueue s')) s' \<and>
+                    sc_at' (the (tcbSchedContext tcb)) s' \<and>
+                    (\<forall>ko. ko_at' ko (the (tcbSchedContext tcb)) s' \<longrightarrow> standard_sc ko)))")
+   apply (safe, blast, blast)[1]
+   apply (rule_tac x=tcb in exI, simp, safe, blast)[1]
+  apply (intro conjI; clarsimp)
+   apply (prop_tac "ksCurThread s' = cur_thread s", clarsimp simp: state_relation_def, simp)
+   apply (rule setNextInterrupt_corres_helper; simp)
+  apply (subgoal_tac "(ksReleaseQueue s') = release_queue s", simp)
+   apply (subgoal_tac "active_sc_tcb_at (hd (release_queue s)) s")
+    apply (rule setNextInterrupt_corres_helper; simp)
+   apply (clarsimp simp: valid_release_q_def)
+  apply (clarsimp simp: state_relation_def release_queue_relation_def)
+  done
+
 lemma schedule_corres:
   "corres dc (invs and valid_sched and valid_list) invs' (Schedule_A.schedule) ThreadDecls_H.schedule"
   supply tcbSchedEnqueue_invs'[wp del]
